termination proof

Examples.thy
@@ -2,7 +2,64 @@ theory Examples
   imports Earley_List
 begin
 
-subsection \<open>Problem 1\<close>
+subsection \<open>Misc Code equations\<close>
+
+fun contains :: "('a \<Rightarrow> bool) \<Rightarrow> 'a list \<Rightarrow> bool" where
+  "contains _ [] = False"
+| "contains f (x#xs) = (if f x then True else contains f xs)"
+
+fun all :: "('a \<Rightarrow> bool) \<Rightarrow> 'a list \<Rightarrow> bool" where
+  "all _ [] = True"
+| "all P (x#xs) \<longleftrightarrow> P x \<and> all P xs"
+
+lemma contains_iff_exists:
+  "contains P xs \<longleftrightarrow> (\<exists>x \<in> set xs. P x)"
+  by (induction xs) auto
+
+lemma all_iff_forall:
+  "all P xs \<longleftrightarrow> (\<forall>x \<in> set xs. P x)"
+  by (induction xs) auto
+
+context Earley_List
+begin
+
+lemma [code]:
+  "is_terminal t = contains (\<lambda>t'. t = t') terminals"
+  using contains_iff_exists is_terminal_def valid_terminals by auto
+
+lemma [code]:
+  "wf_item x = (contains (\<lambda>r. r = item_rule x) rules \<and>
+    item_dot x \<le> length (item_rule_body x) \<and>
+    item_origin x \<le> item_end x \<and>
+    item_end x \<le> length inp)"
+  unfolding wf_item_def using contains_iff_exists valid_rules by auto
+
+lemma [code]:
+  "wf_bin k b = (distinct (items b) \<and> all (\<lambda>x. wf_item x \<and> item_end x = k) (items b))"
+  unfolding wf_bin_def using all_iff_forall by auto
+
+lemma [code]:
+  "wf_bins bs = (all (\<lambda>(k, b). wf_bin k b) (zip [0..<length (bins bs)] (bins bs)))"
+  unfolding wf_bins_def all_iff_forall sorry
+
+(*
+definition wf_item :: "'a item \<Rightarrow> bool" where 
+  "wf_item x = (
+    item_rule x \<in> \<RR> \<and> 
+    item_dot x \<le> length (item_rule_body x) \<and>
+    item_origin x \<le> item_end x \<and> 
+    item_end x \<le> length inp)"
+
+definition wf_bin :: "nat \<Rightarrow> 'a bin \<Rightarrow> bool" where
+  "wf_bin k b \<longleftrightarrow> distinct (items b) \<and> (\<forall>x \<in> set (items b). wf_item x \<and> item_end x = k)"
+
+definition wf_bins :: "'a bins \<Rightarrow> bool" where
+  "wf_bins bs \<longleftrightarrow> (\<forall>k < length (bins bs). wf_bin k (bins bs ! k))"
+*)
+
+end
+
+subsection \<open>Example 1\<close>
 
 (*
 locale CFG =
@@ -35,16 +92,16 @@ definition grammar :: "s rule list" where
     (Nonterminal S, [Nonterminal S, Terminal plus, Nonterminal S])
   ]"
 
-definition terminals :: "s set" where
-  "terminals = {Terminal a, Terminal plus}"
+definition terminals :: "s list" where
+  "terminals = [Terminal a, Terminal plus]"
 
-definition nonterminals :: "s set" where
-  "nonterminals = {Nonterminal S}"
+definition nonterminals :: "s list" where
+  "nonterminals = [Nonterminal S]"
 
 definition inp :: "s list" where
   "inp = [Terminal a]"
 
-global_interpretation earley: Earley_List nonterminals terminals "set grammar" "Nonterminal S" inp grammar
+global_interpretation earley: Earley_List "set nonterminals" "set terminals" "set grammar" "Nonterminal S" inp grammar terminals
   defines init = earley.Init_it
       and scan = earley.Scan_it
       and predict = earley.Predict_it
